defined a new must_movable which considers all the subfields' movability using well-founded recursion; next try to prove its properties

rustfrontend/MoveChecking.v
@@ -6,12 +6,115 @@ Require Import Lattice Kildall.
 Require Import Rusttypes Rustlight Rustlightown RustIR.
 Require Import Errors.
 Require Import InitDomain InitAnalysis RustIRcfg.
+Require Import Wfsimpl.
 
 Import ListNotations.
 Local Open Scope error_monad_scope.
 
+(* A strong must_movable definition to simplify the proof *)
+
+Definition removeR {V: Type} (m1 m2: PTree.t V) :=
+  exists id v, m2 ! id = Some v
+          /\ m1 = PTree.remove id m2.
+
+Lemma well_founded_removeR {V: Type} : well_founded (@removeR V).
+Proof.
+  eapply well_founded_lt_compat with (f := fun m => PTree_Properties.cardinal m).
+  unfold removeR. intros x y (id & v & GET & RM). subst.
+  eapply PTree_Properties.cardinal_remove. eauto.
+Qed.  
+
+Lemma place_neq_Pfield: forall p fid fty, p <> Pfield p fid fty.
+Proof.
+  induction p; intros; try congruence.
+Qed.
+
+Lemma test: forall p1 p2, is_prefix p1 p2 = true -> ~ In p2 (parent_paths p1).
+Proof.
+  induction p1.
+  - admit.
+  - intros. intro. simpl in *.
+    destruct H0. subst. unfold is_prefix in H.
+    destruct place_eq in H; subst.
+    eapply place_neq_Pfield. symmetry. eauto.    
+    erewrite orb_false_l in H.
+    eapply proj_sumbool_true in H.
+    eapply IHp1; eauto. unfold is_prefix.
+    eapply orb_true_intro. right. simpl. destruct place_eq; try congruence.
+    auto.    
+    eapply IHp1; eauto.
+    eapply is_prefix_trans. 2: eauto.
+    unfold is_prefix.
+    eapply orb_true_intro. right. simpl. destruct place_eq; try congruence.
+    auto.
+ Admitted.    
+    
+Lemma is_prefix_not_refl: forall p, ~ In p (parent_paths p).
+Proof.
+  intros.
+  eapply test. apply is_prefix_refl.
+Qed.
+
+Lemma PTree_removeR {V: Type} : forall id v (m: PTree.t V),
+    m ! id = Some v ->
+    removeR (PTree.remove id m) m.
+Proof.
+  intros. red. exists id, v.
+  auto.
+Qed.
+
+Section REC.
+
+  Variable ce: composite_env.
+  Variable rec: forall (ce': composite_env), (removeR ce' ce) -> PathsMap.t -> PathsMap.t -> PathsMap.t -> place -> type -> bool.
+
+  Fixpoint must_movable' (init uninit universe: PathsMap.t) (p: place) (ty: type) : bool :=
+    match ty with
+    | Tbox ty1 =>
+        if must_init init uninit universe p then
+          must_movable' init uninit universe (Pderef p ty1) ty1
+        else false
+    | Tstruct _ id =>
+        match get_composite ce id with
+        | co_some _ i co P =>
+            let fields_types := map (fun '(Member_plain fid fty) => (Pfield p fid fty, fty)) co.(co_members) in
+            (** All sub-fields must be movable *)
+            forallb (fun '(fp, ft) => rec (PTree.remove i ce) (PTree_removeR _ _ _ P) init uninit universe fp ft) fields_types
+        | co_none _ =>
+            (* type error *) false
+        end
+    | Tvariant _ id =>
+        (* may be not required *)
+        match ce ! id with
+        | Some _ =>
+            must_init init uninit universe p
+        | None => false
+        end
+    (* scalar type is movable if it is init *)
+    | Tunit
+    | Tint _ _
+    | Tlong _
+    | Tfloat _ => true
+    (* other types are unsupported to move *)
+    | _ => false
+    end.
+
+End REC.
+  
+(* well_founded_lt_compat *)
+(*   NoDup_incl_length *)
+(*     get_composite *)
+(*     list_norepet implies NoDup *)
+
+(*     PTree.elements_remove *)
+
+Definition must_movable_fix ce := Fix (@well_founded_removeR composite) must_movable' ce.
+
+Definition must_movable ce init uninit universe p := must_movable_fix ce init uninit universe p (typeof_place p).
+
 Section INIT.
 
+Variable ce: composite_env.
 Variable init uninit universe: PathsMap.t.
   
 Fixpoint move_check_pexpr (pe : pexpr) : bool :=
@@ -21,7 +124,9 @@ Fixpoint move_check_pexpr (pe : pexpr) : bool :=
       (* dominators are init means that the location if p is valid;
       the children of p is init means that the value of p is
       semantically wel-typed *)
-      dominators_must_init init uninit universe p && must_movable init uninit universe p
+      (** TODO: in the new must_movable definition, we need to only
+      check the shallow init of this place with scalar type *)
+      dominators_must_init init uninit universe p && must_init init uninit universe p
   | Eref _ _ _ _ => false
   | Eunop _ pe0 _ => move_check_pexpr pe0
   | Ebinop _ pe1 pe2 _ => move_check_pexpr pe1 && move_check_pexpr pe2
@@ -30,7 +135,7 @@ Fixpoint move_check_pexpr (pe : pexpr) : bool :=
   
 Definition move_check_expr (e : expr) :=
   match e with
-  | Emoveplace p _ => dominators_must_init init uninit universe p && must_movable init uninit universe p
+  | Emoveplace p _ => dominators_must_init init uninit universe p && must_movable ce init uninit universe p
   | Epure pe => move_check_pexpr pe
   end.
 
@@ -42,7 +147,7 @@ Definition move_check_assign (p : place) :=
 
 End INIT.
 
-Definition move_check_stmt (an : IM.t * IM.t * PathsMap.t) (stmt : statement) : Errors.res statement :=
+Definition move_check_stmt ce (an : IM.t * IM.t * PathsMap.t) (stmt : statement) : Errors.res statement :=
   let '(mayInit, mayUninit, universe) := an in
   match mayInit, mayUninit with
   | IM.State mayinit, IM.State mayuninit =>      
@@ -50,14 +155,14 @@ Definition move_check_stmt (an : IM.t * IM.t * PathsMap.t) (stmt : statement) : 
       | Sassign p0 e
       | Sassign_variant p0 _ _ e
       | Sbox p0 e =>
-          if move_check_expr mayinit mayuninit universe e
+          if move_check_expr ce mayinit mayuninit universe e
           then
             if move_check_assign mayinit mayuninit universe p0
             then OK stmt
             else Error (msg "move_check_assign error")
           else Error (msg "move_check_expr error")
       | Scall p0 _ el =>
-          if move_check_exprlist mayinit mayuninit universe el
+          if move_check_exprlist ce mayinit mayuninit universe el
           then
             if move_check_assign mayinit mayuninit universe p0
             then OK stmt
@@ -72,7 +177,7 @@ Definition move_check_stmt (an : IM.t * IM.t * PathsMap.t) (stmt : statement) : 
 Definition move_check_function (ce: composite_env) (f: function) : Errors.res unit :=
   do (entry, cfg) <- generate_cfg f.(fn_body);
   do analysis_res <- analyze ce f cfg entry;
-  do _ <- transl_on_cfg get_init_info analysis_res move_check_stmt f.(fn_body) cfg;
+  do _ <- transl_on_cfg get_init_info analysis_res (move_check_stmt ce) f.(fn_body) cfg;
   OK tt.
                                                                     
 Definition transf_fundef (ce : composite_env) (id : ident) (fd : fundef) : Errors.res fundef :=
